Cm/Questions/Sigma2.lean
@@ -2,34 +2,9 @@ import Mathlib.Data.Nat.Notation
 import Mathlib.Tactic
 
 /-
-Realized we've basically been doing sequent calculi the whole time.
+∧ is the equivalent of our ⊢ before.
 
-⊢ : (Prop → Prop) → (Prop → Prop) → Prop → Prop
-
-id α : (∶ Ty α) ∧ ⊢ (snd ∘ fst)
-
-id α : (∶ α) ⊢ (id Prop)
-
-we always want application to produce a judgment.
-This is on normal values, at least.
-
-fst (a ∧ b) = a
-snd (a ∧ b) = b
-
-fst ((∶ m) α a) = ((∶ m.succ) (Ty m) α)
-snd (∶ α m) = (∶ m)
-
-∧ to combine contexts.
-
-We receive our arguments as (∶ T x)
-
-The consequent is the type of the entire application.
-
-I want
-
-id α : (∶ α) ∘ (id Prop) ⊢ (id Prop)
-
-id : (id Prop) ⊢ (∘ (id Prop)) ∘ snd ⊢ (id Prop)
+It combines 
 -/
 
 abbrev Level := ℕ
@@ -40,7 +15,7 @@ inductive Expr where
   | judge : Level → Expr
   | fst   : Expr
   | snd   : Expr
-  | id    : Expr
+  | id    : Level → Expr
   | prop  : Expr
   | comp  : Expr
   | and   : Expr
@@ -56,23 +31,28 @@ syntax "⸨" term+ "⸩"       : term
 notation "Ty" => Expr.ty
 notation "Prp" => Expr.prop
 notation "∶" => Expr.judge
-notation "⊢" => Expr.vdash
 
 macro_rules
   | `(⸨$f:term $x:term⸩) => `(Expr.app $f $x)
   | `(⸨ $f $x:term $args:term*⸩) => `(⸨ (Expr.app $f $x) $args*⸩)
 
-infixr:90 " ∘ " => (fun f g => ⸨Expr.comp f g⸩)
-infixr:90 " ⊢ " => (fun f g => ⸨Expr.vdash f g⸩)
 infixl:90 " ∧ " => (fun f g => ⸨Expr.and f g⸩)
 
+notation "⊢" => Expr.vdash
+notation "∘" => Expr.comp
+
 inductive IsStep : Expr → Expr → Prop
-  | id     : IsStep ⸨Expr.id _α x⸩ x
+  | id     : IsStep ⸨(Expr.id m) _α x⸩ x
   | fst    : IsStep ⸨fst ⸨(∶ m) α x⸩⸩ ⸨(∶ m.succ) (Ty m) α⸩
   | snd    : IsStep ⸨snd ⸨(∶ m.succ) α x⸩⸩ ⸨(∶ m) x⸩
+  | japp   : IsStep ⸨⸨(∶ m) α f⸩ ⸨(∶ n) β x⸩⸩ ⸨(∶ (max m n).succ) ⸨α x⸩ ⸨f x⸩⸩
   | fst'   : IsStep ⸨fst (a ∧ b)⸩ a
-  | snd'   : IsStep ⸨fst (a ∧ b)⸩ b
-  | comp   : IsStep ⸨(f ∘ g) x⸩ ⸨f ⸨g x⸩⸩
+  | snd'   : IsStep ⸨snd (a ∧ b)⸩ b
+  | subst  : IsStep ⸨⸨⊢ α β⸩ x⸩ ⸨⊢ ⸨α x⸩ ⸨β x⸩⸩
+  | fdash  : IsStep ⸨fst ⸨⊢ α β⸩⸩ α
+  | sdash  : IsStep ⸨snd ⸨⊢ α β⸩⸩ β
+  | comp   : IsStep ⸨∘ f g x⸩ ⸨f ⸨g x⸩⸩
+  | const' : IsStep ⸨const' _α _β x y⸩ x
   | left   : IsStep f f'
     → IsStep ⸨f x⸩ ⸨f' x⸩
   | right  : IsStep x x'
@@ -86,18 +66,53 @@ inductive DefEq : Expr → Expr → Prop
   | left    : DefEq f f'  → DefEq ⸨f x⸩ ⸨f' x⸩
   | right   : DefEq x x'  → DefEq ⸨f x⸩ ⸨f x'⸩
 
-def id.type : Expr :=
-  ⸨id Prp⸩ ⊢ (⸨comp ⸨id Prp⸩⸩ ∘ snd) ⊢ ⸨id Prp⸩
+/-
+id : ∀ (α : Type), α → α
+
+id : (const' (Ty m) ⊢ snd ⊢ (id Prp)
+-/
+def id.type (m : Level) : Expr :=
+  ⸨⊢ ⸨(∶ m.succ) (Ty m)⸩ ⸨⊢ snd ⸨(id 0) Prp⸩⸩⸩
 
 inductive ValidJudgment : Typ → Term → Prop
   | ty    : ValidJudgment (Ty m.succ) (Ty m)
   | prp   : ValidJudgment (Ty 0) Prp
-  | app   : ValidJudgment t_x x
-    → ValidJudgment (Ty m) t_x
-    → ValidJudgment (α ⊢ β) f
-    → DefEq ⸨α ⸨(∶ m) t_x x⸩⸩ ⸨(∶ m) t_x x⸩
-    → ValidJudgment ⸨β ⸨(∶ m) t_x x⸩⸩ ⸨f x⸩
-  | defeq : ValidJudgment t₁ e
+  | app   : ValidJudgment t_f f
+    → ValidJudgment ⸨fst ⸨t_f x⸩⸩ x
+    → ValidJudgment ⸨snd ⸨t_f x⸩⸩ ⸨f x⸩
+  | defeq : ValidJudgment ⸨(∶ m) t₁ e⸩ e
     → DefEq t₁ t₂
-    → ValidJudgment t₂ e
+    → ValidJudgment ⸨(∶ m) t₂ e⸩ e
+  | id    : ValidJudgment (id.type m) (id m)
 
+syntax "defeq" ident,*        : tactic
+syntax "step" ident,*         : tactic
+syntax "judge" ident,*         : tactic
+
+macro_rules
+  | `(tactic| defeq $fn:ident,*) => do
+    let nms : Array (Lean.TSyntax `tactic) ← (Array.mk <$> (fn.getElems.toList.mapM (fun name =>
+      let nm := Lean.mkIdent (Lean.Name.mkStr `DefEq name.getId.toString)
+      `(tactic| apply $nm))))
+
+    `(tactic| $[$nms];*)
+  | `(tactic| step $fn:ident,*) => do
+    let nms : Array (Lean.TSyntax `tactic) ← (Array.mk <$> (fn.getElems.toList.mapM (fun name =>
+      let nm := Lean.mkIdent (Lean.Name.mkStr `IsStep name.getId.toString)
+      `(tactic| apply $nm))))
+
+    `(tactic| $[$nms];*)
+  | `(tactic| judge $fn:ident,*) => do
+    let nms : Array (Lean.TSyntax `tactic) ← (Array.mk <$> (fn.getElems.toList.mapM (fun name =>
+      let nm := Lean.mkIdent (Lean.Name.mkStr `ValidJudgment name.getId.toString)
+      `(tactic| apply $nm))))
+
+    `(tactic| $[$nms];*)
+
+theorem id_well_typed : ValidJudgment (Ty m) α
+  → ValidJudgment α x
+  → ValidJudgment ⸨(∶ m) α ⸨(id m) α x⸩ := by
+  intro h_t_α h_t_x
+  judge defeq
+  
+  sorry
